\documentclass[11pt,a4paper]{article}
\usepackage[utf8]{inputenc}
\usepackage[german]{babel}
\usepackage{amsmath}
\usepackage{amsfonts}
\usepackage{amssymb}
\usepackage[left=2cm,right=2cm,top=2cm,bottom=2cm]{geometry}
\begin{document}
.\\
$$Gleichsetzung:$$
$$\frac{\log\frac{y_n}{y_0}}{\log a}=\frac{\log\left(1-\frac{t_n}{t_{max}}\right)}{\log b}$$
$$\Leftrightarrow\log \frac{y_n}{y_0}=\frac{\log a}{\log b}\cdot\log\left(1-\frac{t_n}{t_{max}}\right)$$
$$\Leftrightarrow\log \frac{y_n}{y_0}=\log\left(\left(1-\frac{t_n}{t_{max}}\right)^{\frac{\log a}{\log b}}\right)$$
$$\Leftrightarrow\frac{y_n}{y_0}=\left(1-\frac{t_n}{t_{max}}\right)^{\frac{\log a}{\log b}}$$
$$\Leftrightarrow y_n=y_0\cdot\left(1-\frac{t_n}{t_{max}}\right)^{\frac{\log a}{\log b}}$$
$$y_n=y_0\cdot\left(1-\frac{t_n}{t_{max}}\right)^1$$
\end{document}